SSA/Experimental/Bits/Fast/Defs.lean
@@ -242,19 +242,23 @@ end Predicate
 | .land p q => max p.arity q.arity
 | .neq t₁ t₂ => max t₁.arity t₂.arity
 | .ult t₁ t₂ => max t₁.arity t₂.arity
-| .ule t₁ t₂ => max t₁.arity t₂.arity
+| .ule t₁ t₂ => max (max t₁.arity t₂.arity) (max t₁.arity t₂.arity)
 | .slt t₁ t₂ => max t₁.arity t₂.arity
-| .sle t₁ t₂ => max t₁.arity t₂.arity
+| .sle t₁ t₂ => max (max t₁.arity t₂.arity) (max t₁.arity t₂.arity)
 
+@[simp]
 def Predicate.evalFinLor (x₁ x₂ : BitStream) : BitStream := 
     (x₁ &&& x₂)
 
+@[simp]
 def Predicate.evalFinEq (x₁ x₂ : BitStream) : BitStream := 
     (x₁ ^^^ x₂)
 
+@[simp]
 def Predicate.evalFinSlt (x₁ x₂ : BitStream) : BitStream := 
   ~~~ (x₁ - x₂)
 
+@[simp]
 def Predicate.evalFinUlt (x₁ x₂ : BitStream) : BitStream := 
   (x₁.borrow x₂)
 
